prove hashchain inj bw full chain and bootstrapped chain

new/proof/github_com/sanjit_bhat/pav/hashchain/hashchain.v
@@ -16,45 +16,81 @@ Program Instance is_pkg_init_hashchain : IsPkgInit hashchain := ltac2:(build_pkg
 #[global] Opaque is_pkg_init_hashchain.
 #[local] Transparent is_pkg_init_hashchain.
 
-Local Fixpoint is_chain (l : list $ list w8) (h : list w8) : iProp Σ :=
+Local Fixpoint is_chain_aux (boot : list w8) (l : list $ list w8) (h : list w8) : iProp Σ :=
   match l with
   | [] =>
-    "#His_hash" ∷ cryptoffi.is_hash [] h
+    "->" ∷ ⌜ boot = h ⌝ ∗
+    "%Hlen" ∷ ⌜ Z.of_nat $ length h = cryptoffi.hash_len ⌝
   | x :: l' =>
     ∃ h',
-    "#Hrecur" ∷ is_chain l' h' ∗
+    "#Hrecur" ∷ is_chain_aux boot l' h' ∗
     "#His_hash" ∷ cryptoffi.is_hash (h' ++ x) h
   end.
 
-Local Instance is_chain_pers l h : Persistent (is_chain l h).
-Proof. Admitted.
+#[global]
+Instance is_chain_aux_pers b l h : Persistent (is_chain_aux b l h).
+Proof. revert h. induction l; apply _. Qed.
 
-Lemma is_chain_len l h :
-  is_chain l h -∗
+Lemma is_chain_aux_len b l h :
+  is_chain_aux b l h -∗
   ⌜ Z.of_nat $ length h = cryptoffi.hash_len ⌝.
 Proof.
-  destruct l; simpl; iNamed 1;
-    by iDestruct (cryptoffi.is_hash_len with "His_hash") as %?.
+  destruct l; simpl; iNamed 1.
+  - done.
+  - by iDestruct (cryptoffi.is_hash_len with "His_hash") as %?.
 Qed.
 
-Lemma is_chain_inj l0 l1 h : is_chain l0 h -∗ is_chain l1 h -∗ ⌜ l0 = l1 ⌝.
+(* a full chain. *)
+Definition is_chain l h : iProp Σ :=
+  ∃ he,
+  "#He" ∷ cryptoffi.is_hash [] he ∗
+  "#His_chain" ∷ is_chain_aux he l h.
+
+(* a bootstrapped chain. *)
+Definition is_chain_boot l h : iProp Σ :=
+  ∃ boot,
+  "#His_chain" ∷ is_chain_aux boot l h.
+
+(* we can't prove inj bw two bootstrapped chains bc of cycles.
+i.e., when Hash(boot, v) = boot, which makes
+Chain(boot, []) look indistinguishable from Chain(boot, [v...]).
+one fix is to track a max list limit (XXX: pin down core logic).
+this takes a different approach, stating inj with a "complete"
+chain, which prevents cycles by starting with an empty pre-img. *)
+Lemma is_chain_inj l0 l1 h :
+  is_chain l0 h -∗
+  is_chain_boot l1 h -∗
+  ⌜ l1 `prefix_of` l0 ⌝.
 Proof.
-  iInduction l0 as [|??] forall (l1 h); destruct l1; simpl;
-    iNamedSuffix 1 "0"; iNamedSuffix 1 "1"; try done;
+  iInduction l0 as [|??] forall (l1 h); destruct l1;
+    iNamedSuffix 1 "0"; iNamedSuffix 1 "1"; [done|..]; simpl;
+    iNamedSuffix "His_chain0" "0";
+    iNamedSuffix "His_chain1" "1".
+  - iDestruct (is_chain_aux_len with "Hrecur1") as %?.
+    iDestruct (cryptoffi.is_hash_inj with "He0 His_hash1") as %Heq.
+    apply (f_equal length) in Heq.
+    autorewrite with len in *.
+    word.
+  - iPureIntro. apply prefix_nil.
+  - iDestruct (is_chain_aux_len with "Hrecur0") as %?.
+    iDestruct (is_chain_aux_len with "Hrecur1") as %?.
     iDestruct (cryptoffi.is_hash_inj with "His_hash0 His_hash1") as %Heq.
-  - iDestruct (is_chain_len with "Hrecur1") as %?.
-    apply (f_equal length) in Heq.
-    (* TODO: len tactic should maybe rewrite in *. *)
-    autorewrite with len in *.
-    word.
-  - iDestruct (is_chain_len with "Hrecur0") as %?.
-    apply (f_equal length) in Heq.
-    autorewrite with len in *.
-    word.
-  - iDestruct (is_chain_len with "Hrecur0") as %?.
-    iDestruct (is_chain_len with "Hrecur1") as %?.
     opose proof (app_inj_1 _ _ _ _ _ Heq) as [-> ->]; [lia|].
-    by iDestruct ("IHl0" with "Hrecur0 Hrecur1") as %->.
+    iDestruct ("IHl0" with "[$He0 $Hrecur0] [$Hrecur1]") as %?.
+    iPureIntro. by apply prefix_cons.
+Qed.
+
+Local Lemma is_chain_inj_aux l0 l1 h :
+  is_chain l0 h -∗
+  is_chain l1 h -∗
+  ⌜ l0 = l1 ⌝.
+Proof.
+  iNamedSuffix 1 "0"; iNamedSuffix 1 "1".
+  iDestruct (is_chain_inj with "[$He0 $His_chain0] [$His_chain1]") as %?.
+  iDestruct (is_chain_inj with "[$He1 $His_chain1] [$His_chain0]") as %?.
+  iPureIntro.
+  apply prefix_length_eq; [done|].
+  by apply prefix_length.
 Qed.
 
 End proof.
